SeqPL/Logic/SumQuasiNormal.lean
@@ -7,23 +7,6 @@ public import SeqPL.Formula.Substitution
 @[expose]
 public section
 
-lemma ProvableHilbert.subst {A : Formula α} {s : Formula.Substitution α} (h : ⊢ʰ A) : ⊢ʰ A⟦s⟧ := by
-  induction h using ProvableHilbert.rec with
-  | implyK => exact ProvableHilbert.implyK
-  | implyS => exact ProvableHilbert.implyS
-  | dne => exact ProvableHilbert.dne
-  | andElimL => exact ProvableHilbert.andElimL
-  | andElimR => exact ProvableHilbert.andElimR
-  | andIntro => exact ProvableHilbert.andIntro
-  | orIntroL => exact ProvableHilbert.orIntroL
-  | orIntroR => exact ProvableHilbert.orIntroR
-  | orElim => exact ProvableHilbert.orElim
-  | modalK => exact ProvableHilbert.modalK
-  | modal4 => exact ProvableHilbert.modal4
-  | modalL => exact ProvableHilbert.modalL
-  | mdp h₁ h₂ ih₁ ih₂ => exact ProvableHilbert.mdp ih₁ ih₂
-  | nec h ih => exact ProvableHilbert.nec ih
-
 @[grind]
 inductive Logic.sumQuasiNormal (L₁ L₂ : Logic α) : Logic α
   | mem₁ {A}    : L₁ A → sumQuasiNormal L₁ L₂ A
@@ -34,7 +17,7 @@ infix:50 " +ᴸ " => Logic.sumQuasiNormal
 
 namespace Logic.sumQuasiNormal
 
-variable {L₁ L₂ : Logic α} {A B : Formula α} {s : Formula.Substitution α}
+variable {L₁ L₂ : Logic α} {A B : Formula α} {s : Formula.Substitution α α}
 
 @[grind .] lemma subset_L₁ : L₁ ⊆ (L₁ +ᴸ L₂) := by apply Logic.sumQuasiNormal.mem₁;
 @[grind .] lemma subset_L₂ : L₂ ⊆ (L₁ +ᴸ L₂) := by apply Logic.sumQuasiNormal.mem₂;
